\documentclass{article}
\usepackage{fullpage}
\usepackage{amsmath}
\usepackage{amssymb}

\begin{document}
\section{Rechengesetze f\"ur $\operatorname*{\ast}^{-2}$\newline}

\subsection{}
F\"ur $a, n \in \mathbb{N}$ gilt:
\[ \underbrace{a \operatorname*{\ast}^{-2} \dotsb \operatorname*{\ast}^{-2} a}_n = a\operatorname*{\ast}^{-1} n \]
Da $a\operatorname*{\ast}^{-1}n$ nur f\"ur $a=n=2$ definiert ist, gilt:
\[ \underbrace{a \operatorname*{\ast}^{-2} \dotsb \operatorname*{\ast}^{-2} a}_n = 2\operatorname*{\ast}^{-1}2 \]
Daraus resultiert nach der Definition von $\operatorname*{\ast}^{-1}$:
\[ \underbrace{a \operatorname*{\ast}^{-2} \dotsb \operatorname*{\ast}^{-2} a}_n = 4 \]
\end{document}
